original_work/weight_problems/weighted_problems_poly.thy
@@ -170,4 +170,57 @@ unfolding ispolyred_def
     by blast 
   done 
 
+section "the reduction from subset sum int list to zero one integer programming is polynomial"
+
+definition "ss_int_list_to_zero_one_int_prog_alg \<equiv> \<lambda>(as, s).
+  do {
+    RETURNT ({(as, s)}, as, s)
+  }"
+
+definition "ss_int_list_to_zero_one_int_prog_space n = n"
+definition "ss_int_list_to_zero_one_int_prog_time n = 2 * n + 2"
+
+subsection "proof"
+
+lemma ss_int_list_to_zero_one_int_prog_size:
+"size_zero_one_int_prog (ss_int_list_to_zero_one_int_prog ss) \<le> ss_int_list_to_zero_one_int_prog_space (size_ss_int_list ss)"
+by (auto simp add: size_zero_one_int_prog_def ss_int_list_to_zero_one_int_prog_def 
+ ss_int_list_to_zero_one_int_prog_space_def size_ss_int_list_def)
+
+lemma ss_int_list_to_zero_one_int_prog_refines:
+"ss_int_list_to_zero_one_int_prog_alg ss \<le> SPEC (\<lambda>y. y = ss_int_list_to_zero_one_int_prog ss) 
+  (\<lambda>_. ss_int_list_to_zero_one_int_prog_time (size_ss_int_list ss))"
+unfolding SPEC_def 
+unfolding ss_int_list_to_zero_one_int_prog_alg_def ss_int_list_to_zero_one_int_prog_def 
+apply (rule T_specifies_I)
+apply(vcg' \<open>-\<close> rules: T_SPEC )
+by auto
+
+theorem ss_int_list_to_zero_one_int_prog_is_polyred:
+"ispolyred ss_int_list_to_zero_one_int_prog_alg subset_sum_int_list 
+    zero_one_int_prog size_ss_int_list size_zero_one_int_prog"
+unfolding ispolyred_def
+  apply(rule exI[where x=ss_int_list_to_zero_one_int_prog])
+  apply(rule exI[where x=ss_int_list_to_zero_one_int_prog_time])
+  apply(rule exI[where x=ss_int_list_to_zero_one_int_prog_space])
+  apply safe 
+  subgoal 
+    using ss_int_list_to_zero_one_int_prog_refines
+    by blast
+  subgoal
+    using ss_int_list_to_zero_one_int_prog_size
+    by blast 
+  subgoal 
+    unfolding poly_def ss_int_list_to_zero_one_int_prog_time_def 
+    apply(intro exI[where x=2])
+    by auto
+  subgoal 
+    unfolding poly_def ss_int_list_to_zero_one_int_prog_space_def
+    apply(intro exI[where x=2])
+    by auto
+  subgoal
+    using is_reduction_ss_int_list_to_zero_one_int_prog
+    by blast 
+  done 
+
 end 
