original_work/weight_problems/weighted_problems.thy
@@ -321,5 +321,22 @@ theorem is_reduction_ss_to_ks:
   using ss_to_ks_sound ss_to_ks_complete 
   by fast
 
+subsection "the reduction from subset sum int list to zero one integer programming is correct"
 
-end 
+lemma ss_int_list_to_zero_one_int_prog_sound:
+"(as, s) \<in> subset_sum_int_list \<Longrightarrow> ({(as, s)}, as, s) \<in> zero_one_int_prog"
+unfolding subset_sum_int_list_def zero_one_int_prog_def 
+by blast 
+
+lemma ss_int_list_to_zero_one_int_prog_complete:
+"({(as, s)}, as, s) \<in> zero_one_int_prog \<Longrightarrow> (as, s) \<in> subset_sum_int_list"
+unfolding subset_sum_int_list_def zero_one_int_prog_def 
+by auto
+
+theorem is_reduction_ss_int_list_to_zero_one_int_prog:
+"is_reduction ss_int_list_to_zero_one_int_prog subset_sum_int_list zero_one_int_prog"
+unfolding is_reduction_def ss_int_list_to_zero_one_int_prog_def 
+using ss_int_list_to_zero_one_int_prog_sound ss_int_list_to_zero_one_int_prog_complete 
+by auto
+
+end
